- try new worklist_subst

proof/old_system/uni/algo_worklist/def_extra.v
@@ -74,6 +74,38 @@ Inductive aworklist_subst : aworklist -> typvar -> typ ->  list typvar -> aworkl
         aworklist_subst (aworklist_constvar Γ Y (abind_etvar_empty)) X A (Y :: E) Γ1 Γ2
     .
 
+    
+Inductive aworklist_subst' : aworklist -> typvar -> typ -> aworklist -> aworklist -> Prop :=
+| a_ws1__stop : forall Γ X A , 
+    aworklist_subst' (aworklist_constvar Γ X (abind_etvar_empty)) X A Γ aworklist_empty
+| a_ws1__var_stay : forall Γ X Y A B Γ1 Γ2,
+    aworklist_subst' Γ X A Γ1 Γ2 ->
+    aworklist_subst' (aworklist_consvar Γ Y (abind_var_typ B)) X A Γ1 (aworklist_consvar Γ2 Y (abind_var_typ B))
+| a_ws1__tvar_stay : forall Γ X Y A Γ1 Γ2,
+    aworklist_subst' Γ X A Γ1 Γ2 ->
+    Y <> X ->
+    Y `notin` ftvar_in_typ A -> 
+    aworklist_subst' (aworklist_constvar Γ Y (abind_tvar_empty)) X A Γ1 (aworklist_constvar Γ2 Y (abind_tvar_empty))
+| a_ws1__stvar_stay : forall Γ X Y A Γ1 Γ2,
+    aworklist_subst' Γ X A Γ1 Γ2 ->
+    Y <> X ->
+    Y `notin` ftvar_in_typ A -> 
+    aworklist_subst' (aworklist_constvar Γ Y (abind_stvar_empty)) X A Γ1 (aworklist_constvar Γ2 Y (abind_stvar_empty))
+| a_ws1__work_stay : forall Γ X A w Γ1 Γ2,
+    aworklist_subst' Γ X A Γ1 Γ2 ->
+    aworklist_subst' (aworklist_conswork Γ w) X A  Γ1 (aworklist_conswork Γ2 w)
+| a_ws1__etvar_stay : forall Γ X Y A Γ1 Γ2,
+    aworklist_subst' Γ X A Γ1 Γ2 ->
+    Y <> X ->
+    Y `notin` ftvar_in_typ A -> 
+    aworklist_subst' (aworklist_constvar Γ Y (abind_etvar_empty)) X A Γ1 (aworklist_constvar Γ2 Y (abind_etvar_empty))
+| a_ws1__etvar_move : forall Γ1 Γ2 X Y A  Γ'1 Γ'2,
+    aworklist_subst' (awl_app Γ2 (aworklist_constvar (aworklist_constvar Γ1 Y abind_etvar_empty) X abind_etvar_empty)) X A Γ'1 Γ'2 ->
+    Y <> X ->
+    Y `in` ftvar_in_typ A -> 
+    aworklist_subst' (aworklist_constvar (awl_app Γ2 (aworklist_constvar Γ1 X abind_etvar_empty)) Y (abind_etvar_empty)) X A Γ'1 Γ'2
+.
+    
 
 (* defns Jaworklist_reduction *)
 Inductive a_wl_red : aworklist -> Prop :=    (* defn a_wl_red *)
